contrib/correctness/Exchange.v
@@ -25,23 +25,23 @@ Implicit Arguments On.
 Inductive exchange [n:Z; A:Set; t,t':(array n A); i,j:Z] : Prop :=
   exchange_c :
     `0<=i<n` -> `0<=j<n` ->
-    (t#[i] = t'#[j]) ->
-    (t#[j] = t'#[i]) ->
-    ((k:Z)`0<=k<n` -> `k<>i` -> `k<>j` -> t#[k] = t'#[k]) ->
+    (#t[i] = #t'[j]) ->
+    (#t[j] = #t'[i]) ->
+    ((k:Z)`0<=k<n` -> `k<>i` -> `k<>j` -> #t[k] = #t'[k]) ->
     (exchange t t' i j).
     
 (* Properties about exchanges *)
 
 Lemma exchange_1 : (n:Z)(A:Set)(t:(array n A))
   (i,j:Z) `0<=i<n` -> `0<=j<n` ->
-  (access (store (store t i t#[j]) j t#[i]) i)=t#[j].
+  (access (store (store t i #t[j]) j #t[i]) i) = #t[j].
 Proof.
 Intros n A t i j H_i H_j.
 Case (dec_eq j i).
 Intro eq_i_j. Rewrite eq_i_j.
 Auto with datatypes.
 Intro not_j_i.
-Rewrite (store_def_2 (store t i t#[j]) t#[i] H_j H_i not_j_i).
+Rewrite (store_def_2 (store t i #t[j]) #t[i] H_j H_i not_j_i).
 Auto with datatypes.
 Save.
 
