.depend.coq
@@ -160,10 +160,10 @@ contrib/omega/Omega.vo: contrib/omega/Omega.v theories/Zarith/ZArith.vo theories
 contrib/interface/Centaur.vo: contrib/interface/Centaur.v contrib/interface/paths.cmo contrib/interface/name_to_ast.cmo contrib/interface/xlate.cmo contrib/interface/vtp.cmo contrib/interface/translate.cmo contrib/interface/pbp.cmo contrib/interface/dad.cmo contrib/interface/debug_tac.cmo contrib/interface/history.cmo contrib/interface/centaur.cmo contrib/interface/AddDad.vo
 contrib/interface/AddDad.vo: contrib/interface/AddDad.v
 contrib/extraction/test_extraction.vo: contrib/extraction/test_extraction.v
-contrib/extraction/Extraction.vo: contrib/extraction/Extraction.v
+contrib/extraction/Extraction.vo: contrib/extraction/Extraction.v contrib/extraction/mlutil.cmo contrib/extraction/ocaml.cmo contrib/extraction/extraction.cmo contrib/extraction/extract_env.cmo
 contrib/correctness/preuves.vo: contrib/correctness/preuves.v contrib/omega/Omega.vo
 contrib/correctness/Tuples.vo: contrib/correctness/Tuples.v
-contrib/correctness/Sorted.vo: contrib/correctness/Sorted.v contrib/correctness/Arrays.vo theories/Sets/Permut.vo contrib/ring/ZArithRing.vo contrib/omega/Omega.vo
+contrib/correctness/Sorted.vo: contrib/correctness/Sorted.v contrib/correctness/Arrays.vo contrib/correctness/ArrayPermut.vo contrib/ring/ZArithRing.vo contrib/omega/Omega.vo
 contrib/correctness/Programs_stuff.vo: contrib/correctness/Programs_stuff.v contrib/correctness/Arrays_stuff.vo
 contrib/correctness/ProgramsExtraction.vo: contrib/correctness/ProgramsExtraction.v contrib/extraction/Extraction.vo
 contrib/correctness/ProgWf.vo: contrib/correctness/ProgWf.v theories/Zarith/ZArith.vo theories/Arith/Wf_nat.vo
@@ -172,8 +172,8 @@ contrib/correctness/ProgBool.vo: contrib/correctness/ProgBool.v theories/Arith/C
 contrib/correctness/Permut.vo: contrib/correctness/Permut.v contrib/correctness/ProgInt.vo contrib/correctness/Arrays.vo contrib/correctness/Exchange.vo contrib/omega/Omega.vo
 contrib/correctness/MakeProgramsState.vo: contrib/correctness/MakeProgramsState.v
 contrib/correctness/Exchange.vo: contrib/correctness/Exchange.v contrib/correctness/ProgInt.vo contrib/correctness/Arrays.vo
-contrib/correctness/Correctness.vo: contrib/correctness/Correctness.v tactics/Refine.vo contrib/correctness/Tuples.vo contrib/correctness/ProgInt.vo contrib/correctness/ProgBool.vo contrib/correctness/ProgWf.vo contrib/correctness/Arrays.vo contrib/correctness/pmisc.cmo contrib/correctness/peffect.cmo contrib/correctness/prename.cmo contrib/correctness/ptype.cmo contrib/correctness/past.cmo contrib/correctness/perror.cmo contrib/correctness/penv.cmo contrib/correctness/putil.cmo contrib/correctness/pdb.cmo contrib/correctness/pcic.cmo contrib/correctness/pmonad.cmo contrib/correctness/pcicenv.cmo contrib/correctness/pred.cmo contrib/correctness/ptyping.cmo contrib/correctness/pwp.cmo contrib/correctness/pmlize.cmo contrib/correctness/ptactic.cmo contrib/correctness/psyntax.cmo
-contrib/correctness/Arrays_stuff.vo: contrib/correctness/Arrays_stuff.v contrib/correctness/Exchange.vo theories/Sets/Permut.vo contrib/correctness/Sorted.vo
+contrib/correctness/Correctness.vo: contrib/correctness/Correctness.v tactics/Refine.vo contrib/correctness/Tuples.vo contrib/correctness/ProgInt.vo contrib/correctness/ProgBool.vo contrib/correctness/ProgWf.vo contrib/correctness/Arrays.vo contrib/correctness/pmisc.cmo contrib/correctness/peffect.cmo contrib/correctness/prename.cmo contrib/correctness/perror.cmo contrib/correctness/penv.cmo contrib/correctness/putil.cmo contrib/correctness/pdb.cmo contrib/correctness/pcic.cmo contrib/correctness/pmonad.cmo contrib/correctness/pcicenv.cmo contrib/correctness/pred.cmo contrib/correctness/ptyping.cmo contrib/correctness/pwp.cmo contrib/correctness/pmlize.cmo contrib/correctness/ptactic.cmo contrib/correctness/psyntax.cmo
+contrib/correctness/Arrays_stuff.vo: contrib/correctness/Arrays_stuff.v contrib/correctness/Exchange.vo contrib/correctness/Permut.vo contrib/correctness/Sorted.vo
 contrib/correctness/Arrays.vo: contrib/correctness/Arrays.v contrib/correctness/ProgInt.vo
 tactics/Tauto.vo: tactics/Tauto.v
 tactics/Refine.vo: tactics/Refine.v
@@ -189,20 +189,23 @@ syntax/MakeBare.vo: syntax/MakeBare.v
 states/MakeInitial.vo: states/MakeInitial.v theories/Init/Prelude.vo theories/Init/Logic_Type.vo theories/Init/Logic_TypeSyntax.vo tactics/Equality.vo test-suite/success/Tauto.vo tactics/Inv.vo tactics/EAuto.vo tactics/AutoRewrite.vo tactics/Refine.vo tactics/EqDecide.vo
 contrib/interface/Centaur.vo: contrib/interface/Centaur.v contrib/interface/paths.cmo contrib/interface/name_to_ast.cmo contrib/interface/xlate.cmo contrib/interface/vtp.cmo contrib/interface/translate.cmo contrib/interface/pbp.cmo contrib/interface/dad.cmo contrib/interface/debug_tac.cmo contrib/interface/history.cmo contrib/interface/centaur.cmo contrib/interface/AddDad.vo
 contrib/interface/AddDad.vo: contrib/interface/AddDad.v
+contrib/correctness/Correctness.vo: contrib/correctness/Correctness.v tactics/Refine.vo contrib/correctness/Tuples.vo contrib/correctness/ProgInt.vo contrib/correctness/ProgBool.vo contrib/correctness/ProgWf.vo contrib/correctness/Arrays.vo contrib/correctness/pmisc.cmo contrib/correctness/peffect.cmo contrib/correctness/prename.cmo contrib/correctness/perror.cmo contrib/correctness/penv.cmo contrib/correctness/putil.cmo contrib/correctness/pdb.cmo contrib/correctness/pcic.cmo contrib/correctness/pmonad.cmo contrib/correctness/pcicenv.cmo contrib/correctness/pred.cmo contrib/correctness/ptyping.cmo contrib/correctness/pwp.cmo contrib/correctness/pmlize.cmo contrib/correctness/ptactic.cmo contrib/correctness/psyntax.cmo
+contrib/correctness/ProgWf.vo: contrib/correctness/ProgWf.v theories/Zarith/ZArith.vo theories/Arith/Wf_nat.vo
+contrib/correctness/Programs_stuff.vo: contrib/correctness/Programs_stuff.v contrib/correctness/Arrays_stuff.vo
+contrib/correctness/ProgramsExtraction.vo: contrib/correctness/ProgramsExtraction.v contrib/extraction/Extraction.vo
+contrib/correctness/ProgInt.vo: contrib/correctness/ProgInt.v theories/Zarith/ZArith.vo theories/Zarith/ZArith_dec.vo
+contrib/correctness/ProgBool.vo: contrib/correctness/ProgBool.v theories/Arith/Compare_dec.vo theories/Arith/Peano_dec.vo theories/Zarith/ZArith.vo theories/Bool/Sumbool.vo
 contrib/correctness/preuves.vo: contrib/correctness/preuves.v contrib/omega/Omega.vo
+contrib/correctness/Permut.vo: contrib/correctness/Permut.v contrib/correctness/ProgInt.vo contrib/correctness/Arrays.vo contrib/correctness/Exchange.vo contrib/omega/Omega.vo
+contrib/correctness/MakeProgramsState.vo: contrib/correctness/MakeProgramsState.v
+contrib/correctness/Exchange.vo: contrib/correctness/Exchange.v contrib/correctness/ProgInt.vo contrib/correctness/Arrays.vo
+contrib/correctness/Arrays.vo: contrib/correctness/Arrays.v contrib/correctness/ProgInt.vo
+contrib/correctness/Arrays_stuff.vo: contrib/correctness/Arrays_stuff.v contrib/correctness/Exchange.vo contrib/correctness/Permut.vo contrib/correctness/Sorted.vo
 contrib/correctness/Tuples.vo: contrib/correctness/Tuples.v
 contrib/correctness/Sorted.vo: contrib/correctness/Sorted.v contrib/correctness/Arrays.vo theories/Sets/Permut.vo contrib/ring/ZArithRing.vo contrib/omega/Omega.vo
-contrib/correctness/Programs_stuff.vo: contrib/correctness/Programs_stuff.v contrib/correctness/Arrays_stuff.vo
-contrib/correctness/ProgWf.vo: contrib/correctness/ProgWf.v theories/Zarith/ZArith.vo theories/Arith/Wf_nat.vo
-contrib/correctness/ProgInt.vo: contrib/correctness/ProgInt.v theories/Zarith/ZArith.vo theories/Zarith/ZArith_dec.vo
-contrib/correctness/ProgramsExtraction.vo: contrib/correctness/ProgramsExtraction.v contrib/extraction/Extraction.vo
-contrib/correctness/Permut.vo: contrib/correctness/Permut.v contrib/correctness/ProgInt.vo contrib/correctness/Arrays.vo contrib/correctness/Exchange.vo contrib/omega/Omega.vo
-contrib/correctness/ProgBool.vo: contrib/correctness/ProgBool.v theories/Arith/Compare_dec.vo theories/Arith/Peano_dec.vo theories/Zarith/ZArith.vo theories/Bool/Sumbool.vo
-contrib/correctness/Exchange.vo: contrib/correctness/Exchange.v contrib/correctness/ProgInt.vo contrib/correctness/Arrays.vo
-contrib/correctness/Correctness.vo: contrib/correctness/Correctness.v tactics/Refine.vo contrib/correctness/Tuples.vo contrib/correctness/ProgInt.vo contrib/correctness/ProgBool.vo contrib/correctness/ProgWf.vo contrib/correctness/Arrays.vo contrib/correctness/pmisc.cmo contrib/correctness/peffect.cmo contrib/correctness/prename.cmo contrib/correctness/ptype.cmo contrib/correctness/past.cmo contrib/correctness/perror.cmo contrib/correctness/penv.cmo contrib/correctness/putil.cmo contrib/correctness/pdb.cmo contrib/correctness/pcic.cmo contrib/correctness/pmonad.cmo contrib/correctness/pcicenv.cmo contrib/correctness/pred.cmo contrib/correctness/ptyping.cmo contrib/correctness/pwp.cmo contrib/correctness/pmlize.cmo contrib/correctness/ptactic.cmo contrib/correctness/psyntax.cmo
-contrib/correctness/MakeProgramsState.vo: contrib/correctness/MakeProgramsState.v
-contrib/correctness/Arrays.vo: contrib/correctness/Arrays.v contrib/correctness/ProgInt.vo
-contrib/correctness/Arrays_stuff.vo: contrib/correctness/Arrays_stuff.v contrib/correctness/Exchange.vo theories/Sets/Permut.vo contrib/correctness/Sorted.vo
+contrib/extraction/test/bench.vo: contrib/extraction/test/bench.v theories/Lists/PolyList.vo theories/Zarith/ZArith.vo theories/Arith/Even.vo
+contrib/extraction/test_extraction.vo: contrib/extraction/test_extraction.v
+contrib/extraction/Extraction.vo: contrib/extraction/Extraction.v contrib/extraction/mlutil.cmo contrib/extraction/ocaml.cmo contrib/extraction/extraction.cmo contrib/extraction/extract_env.cmo
 contrib/xml/Xml.vo: contrib/xml/Xml.v contrib/xml/xml.cmo contrib/xml/xmlcommand.cmo contrib/xml/xmlentries.cmo
 contrib/ring/ZArithRing.vo: contrib/ring/ZArithRing.v contrib/ring/ArithRing.vo theories/Zarith/ZArith.vo theories/Logic/Eqdep_dec.vo
 contrib/ring/Ring_theory.vo: contrib/ring/Ring_theory.v theories/Bool/Bool.vo
@@ -216,9 +219,32 @@ contrib/omega/Zcomplements.vo: contrib/omega/Zcomplements.v theories/Zarith/ZAri
 contrib/omega/OmegaSyntax.vo: contrib/omega/OmegaSyntax.v
 contrib/omega/Omega.vo: contrib/omega/Omega.v theories/Zarith/ZArith.vo theories/Arith/Minus.vo contrib/omega/omega.cmo contrib/omega/coq_omega.cmo contrib/omega/OmegaSyntax.vo
 contrib/omega/Zlogarithm.vo: contrib/omega/Zlogarithm.v theories/Zarith/ZArith.vo contrib/omega/Omega.vo contrib/omega/Zcomplements.vo contrib/omega/Zpower.vo
-contrib/extraction/test_extraction.vo: contrib/extraction/test_extraction.v
-contrib/extraction/Extraction.vo: contrib/extraction/Extraction.v
-contrib/extraction/test/bench.vo: contrib/extraction/test/bench.v theories/Lists/PolyList.vo theories/Zarith/ZArith.vo theories/Arith/Even.vo
+theories/Num/Nat/NeqDef.vo: theories/Num/Nat/NeqDef.v theories/Num/Params.vo
+theories/Num/Nat/NSyntax.vo: theories/Num/Nat/NSyntax.v
+theories/Num/Nat/Axioms.vo: theories/Num/Nat/Axioms.v theories/Num/Params.vo theories/Num/EqAxioms.vo theories/Num/NSyntax.vo
+theories/Num/Params.vo: theories/Num/Params.v
+theories/Num/NeqDef.vo: theories/Num/NeqDef.v theories/Num/Params.vo theories/Num/EqParams.vo
+theories/Num/EqParams.vo: theories/Num/EqParams.v theories/Num/Params.vo
+theories/Num/EqAxioms.vo: theories/Num/EqAxioms.v theories/Num/Params.vo theories/Num/EqParams.vo theories/Num/NeqDef.vo theories/Num/NSyntax.vo
+theories/Num/SubProps.vo: theories/Num/SubProps.v
+theories/Num/OppProps.vo: theories/Num/OppProps.v
+theories/Num/OppAxioms.vo: theories/Num/OppAxioms.v
+theories/Num/NSyntax.vo: theories/Num/NSyntax.v theories/Num/Params.vo
+theories/Num/LtProps.vo: theories/Num/LtProps.v theories/Num/Axioms.vo theories/Num/AddProps.vo
+theories/Num/LeProps.vo: theories/Num/LeProps.v theories/Num/LtProps.vo theories/Num/LeAxioms.vo
+theories/Num/LeAxioms.vo: theories/Num/LeAxioms.v theories/Num/Axioms.vo theories/Num/LtProps.vo
+theories/Num/GtProps.vo: theories/Num/GtProps.v
+theories/Num/GtAxioms.vo: theories/Num/GtAxioms.v theories/Num/Axioms.vo theories/Num/LeProps.vo
+theories/Num/GeProps.vo: theories/Num/GeProps.v
+theories/Num/GeAxioms.vo: theories/Num/GeAxioms.v theories/Num/Axioms.vo theories/Num/LtProps.vo
+theories/Num/DiscrProps.vo: theories/Num/DiscrProps.v theories/Num/DiscrAxioms.vo theories/Num/LtProps.vo
+theories/Num/Leibniz/Params.vo: theories/Num/Leibniz/Params.v
+theories/Num/Leibniz/NSyntax.vo: theories/Num/Leibniz/NSyntax.v theories/Num/Params.vo
+theories/Num/Leibniz/EqAxioms.vo: theories/Num/Leibniz/EqAxioms.v theories/Num/NSyntax.vo
+theories/Num/DiscrAxioms.vo: theories/Num/DiscrAxioms.v theories/Num/Params.vo theories/Num/NSyntax.vo
+theories/Num/Axioms.vo: theories/Num/Axioms.v theories/Num/Params.vo theories/Num/EqParams.vo theories/Num/NeqDef.vo theories/Num/NSyntax.vo
+theories/Num/AddProps.vo: theories/Num/AddProps.v theories/Num/Axioms.vo theories/Num/EqAxioms.vo
+theories/Num/Definitions.vo: theories/Num/Definitions.v
 theories/Zarith/zarith_aux.vo: theories/Zarith/zarith_aux.v theories/Arith/Arith.vo theories/Zarith/fast_integer.vo
 theories/Zarith/fast_integer.vo: theories/Zarith/fast_integer.v theories/Arith/Le.vo theories/Arith/Lt.vo theories/Arith/Plus.vo theories/Arith/Mult.vo theories/Arith/Minus.vo
 theories/Zarith/auxiliary.vo: theories/Zarith/auxiliary.v theories/Arith/Arith.vo theories/Zarith/fast_integer.vo theories/Zarith/zarith_aux.vo theories/Arith/Peano_dec.vo theories/Arith/Compare_dec.vo
@@ -275,32 +301,6 @@ theories/Reals/Rbase.vo: theories/Reals/Rbase.v theories/Reals/Raxioms.vo contri
 theories/Reals/Rbasic_fun.vo: theories/Reals/Rbasic_fun.v theories/Reals/R_Ifp.vo
 theories/Reals/R_Ifp.vo: theories/Reals/R_Ifp.v theories/Reals/Rbase.vo contrib/omega/Omega.vo
 theories/Reals/Raxioms.vo: theories/Reals/Raxioms.v theories/Zarith/ZArith.vo theories/Reals/Rsyntax.vo theories/Reals/TypeSyntax.vo
-theories/Num/Params.vo: theories/Num/Params.v
-theories/Num/NeqDef.vo: theories/Num/NeqDef.v theories/Num/Params.vo theories/Num/EqParams.vo
-theories/Num/EqParams.vo: theories/Num/EqParams.v theories/Num/Params.vo
-theories/Num/EqAxioms.vo: theories/Num/EqAxioms.v theories/Num/Params.vo theories/Num/EqParams.vo theories/Num/NeqDef.vo theories/Num/NSyntax.vo
-theories/Num/Nat/NeqDef.vo: theories/Num/Nat/NeqDef.v theories/Num/Params.vo
-theories/Num/Nat/Axioms.vo: theories/Num/Nat/Axioms.v theories/Num/Params.vo theories/Num/EqAxioms.vo theories/Num/NSyntax.vo
-theories/Num/Nat/NSyntax.vo: theories/Num/Nat/NSyntax.v
-theories/Num/SubProps.vo: theories/Num/SubProps.v
-theories/Num/OppProps.vo: theories/Num/OppProps.v
-theories/Num/OppAxioms.vo: theories/Num/OppAxioms.v
-theories/Num/NSyntax.vo: theories/Num/NSyntax.v theories/Num/Params.vo
-theories/Num/LtProps.vo: theories/Num/LtProps.v theories/Num/Axioms.vo theories/Num/AddProps.vo
-theories/Num/LeProps.vo: theories/Num/LeProps.v theories/Num/LtProps.vo theories/Num/LeAxioms.vo
-theories/Num/LeAxioms.vo: theories/Num/LeAxioms.v theories/Num/Axioms.vo theories/Num/LtProps.vo
-theories/Num/GtProps.vo: theories/Num/GtProps.v
-theories/Num/GtAxioms.vo: theories/Num/GtAxioms.v theories/Num/Axioms.vo theories/Num/LeProps.vo
-theories/Num/GeProps.vo: theories/Num/GeProps.v
-theories/Num/GeAxioms.vo: theories/Num/GeAxioms.v theories/Num/Axioms.vo theories/Num/LtProps.vo
-theories/Num/DiscrProps.vo: theories/Num/DiscrProps.v theories/Num/DiscrAxioms.vo theories/Num/LtProps.vo
-theories/Num/DiscrAxioms.vo: theories/Num/DiscrAxioms.v theories/Num/Params.vo theories/Num/NSyntax.vo
-theories/Num/Definitions.vo: theories/Num/Definitions.v
-theories/Num/Axioms.vo: theories/Num/Axioms.v theories/Num/Params.vo theories/Num/EqParams.vo theories/Num/NeqDef.vo theories/Num/NSyntax.vo
-theories/Num/AddProps.vo: theories/Num/AddProps.v theories/Num/Axioms.vo theories/Num/EqAxioms.vo
-theories/Num/Leibniz/Params.vo: theories/Num/Leibniz/Params.v
-theories/Num/Leibniz/NSyntax.vo: theories/Num/Leibniz/NSyntax.v theories/Num/Params.vo
-theories/Num/Leibniz/EqAxioms.vo: theories/Num/Leibniz/EqAxioms.v theories/Num/NSyntax.vo
 theories/Logic/Eqdep_dec.vo: theories/Logic/Eqdep_dec.v
 theories/Logic/Eqdep.vo: theories/Logic/Eqdep.v
 theories/Logic/Classical_Type.vo: theories/Logic/Classical_Type.v theories/Logic/Classical_Prop.vo theories/Logic/Classical_Pred_Type.vo
